src/Examples/ExMach/RefinementAdequacy.v
@@ -117,11 +117,8 @@ Module exmach_refinement (eRT: exmach_refinement_type).
     Definition set_inv_reg Hex Hinv Hreg :=
       ExMachG Σ Hinv (@exm_mem_inG _ Hex) (@exm_disk_inG _ Hex) Hreg.
 
-    (* N.B. this definition reads funny, but it's to match the way ExMach
-       refinement adequacy was done before, probably for most layers going
-       forward the definition would be crash_inner := crash_inner *)
-    Definition crash_inner : cfgG eRT.Σ → WeakestPre.exmachG eRT.Σ → iProp eRT.Σ
-      := (λ H1 H2, ∃ Hinv Hreg, crash_inner H1 (set_inv_reg H2 Hinv Hreg))%I.
+    Definition crash_inner := crash_inner. (* : cfgG eRT.Σ → WeakestPre.exmachG eRT.Σ → iProp eRT.Σ
+      := (λ H1 H2, ∃ Hinv Hreg, crash_inner H1 (set_inv_reg H2 Hinv Hreg))%I. *)
 
     Definition exec_inner := exec_inner.
     Definition crash_inv := crash_inv.
@@ -150,6 +147,11 @@ Module exmach_refinement (eRT: exmach_refinement_type).
     Import WeakestPre.
     Import RT RD.
 
+    Lemma set_inv_reg_spec0:
+             ∀ Hex, (set_inv_reg Hex (Hinstance Σ Hex).(@iris_invG OpC (State Λc) Σ)
+                                                         (Hinstance_reg Σ Hex) = Hex).
+    Proof. destruct Hex; auto. Qed.
+
     Lemma set_inv_reg_spec1:
       ∀ Hex Hinv Hreg, @iris_invG _ _ _ (Hinstance _ (set_inv_reg Hex Hinv Hreg)) = Hinv.
     Proof. trivial. Qed.
@@ -159,7 +161,7 @@ Module exmach_refinement (eRT: exmach_refinement_type).
     Proof. trivial. Qed.
 
     Lemma set_inv_reg_spec3:
-      ∀ Hex Hinv Hreg, set_inv_reg (set_inv_reg Hex Hinv Hreg) Hinv Hreg =
+      ∀ Hex Hinv Hinv' Hreg Hreg', set_inv_reg (set_inv_reg Hex Hinv' Hreg') Hinv Hreg =
                        (set_inv_reg Hex Hinv Hreg).
     Proof. trivial. Qed.
 
@@ -216,25 +218,23 @@ Module exmach_refinement (eRT: exmach_refinement_type).
     iIntros (??) "Hinv".
     iPoseProof (eRT.exec_inv_preserve_crash with "Hinv") as "Hinv_post".
     iMod (gen_heap_strong_init (init_zero)) as (hM Hmpf_eq) "(Hmc&Hm)".
-    iMod (own_alloc (Cinl (Count 0))) as (tR_fresh) "Ht".
-    { constructor. }
-    set (tR := {| treg_name := tR_fresh; treg_counter_inG := _ |}).
+    iMod ("Hinv_post") as "Hinv_post".
+    iModIntro. iIntros (?).
     iMod ("Hinv_post" with "[Hm]") as "Hinv_post".
     { rewrite -Hmpf_eq. iApply @mem_init_to_bigOp; auto. }
-    iMod "Hinv_post". iModIntro.
-    iIntros (n σ σ' Hcrash ??) "(Hmach&Hthread)".
-    iExists (ExMachG Σ a hM (@exm_disk_inG _ Hex)
+    iModIntro.
+    iIntros (n σ σ' Hcrash) "(Hmach&Hthread)".
+    iExists (ExMachG Σ (@exm_invG _ Hex) hM (@exm_disk_inG _ Hex)
                      (@exm_treg_inG _ Hex)).
     iModIntro. iFrame. iDestruct "Hmach" as "(?&Hdisk)".
     inversion Hcrash. subst.
     iDestruct "Hdisk" as (??) "(?&?&%&%&%&%)". iFrame.
-    iSplitR "Hinv_post".
-    - iExists _, _. iFrame.
-      iPureIntro; split_and!; [ auto | auto | | assumption ].
-      intros ? Hsome. apply not_le; intros Hge.
-      rewrite init_zero_lookup_ge_None in Hsome; last by lia.
-      apply is_Some_None in Hsome; auto.
-    - by iExists (@exm_invG _ Hex), tR.
+    iSplitR ""; last done.
+    iExists _, _. iFrame.
+    iPureIntro; split_and!; [ auto | auto | | assumption ].
+    intros ? Hsome. apply not_le; intros Hge.
+    rewrite init_zero_lookup_ge_None in Hsome; last by lia.
+    apply is_Some_None in Hsome; auto.
   Qed.
 
   Lemma crash_inv_preserve_crash: crash_inv_preserve_crash_type.
@@ -243,452 +243,76 @@ Module exmach_refinement (eRT: exmach_refinement_type).
     iIntros (???) "Hinv".
     iPoseProof (eRT.crash_inv_preserve_crash with "Hinv") as "Hinv_post".
     iMod (gen_heap_strong_init (init_zero)) as (hM Hmpf_eq) "(Hmc&Hm)".
-    iMod (own_alloc (Cinl (Count 0))) as (tR_fresh) "Ht".
-    { constructor. }
-    set (tR := {| treg_name := tR_fresh; treg_counter_inG := _ |}).
+    iMod ("Hinv_post") as "Hinv_post".
+    iModIntro. iIntros (?).
     iMod ("Hinv_post" with "[Hm]") as "Hinv_post".
     { rewrite -Hmpf_eq. iApply @mem_init_to_bigOp; auto. }
-    iMod "Hinv_post". iModIntro.
-    iIntros (n σ σ' Hcrash ??) "(Hmach&Hthread)".
-    iExists (ExMachG Σ a hM (@exm_disk_inG _ Hex)
+    iModIntro.
+    iIntros (n σ σ' Hcrash) "(Hmach&Hthread)".
+    iExists (ExMachG Σ (@exm_invG _ Hex) hM (@exm_disk_inG _ Hex)
                      (@exm_treg_inG _ Hex)).
     iModIntro. iFrame. iDestruct "Hmach" as "(?&Hdisk)".
     inversion Hcrash. subst.
     iDestruct "Hdisk" as (??) "(?&?&%&%&%&%)". iFrame.
-    iSplitR "Hinv_post".
-    - iExists _, _. iFrame.
+    iSplitR ""; last done.
+    iExists _, _. iFrame.
+    iPureIntro; split_and!; [ auto | auto | | assumption ].
+    intros ? Hsome. apply not_le; intros Hge.
+    rewrite init_zero_lookup_ge_None in Hsome; last by lia.
+    apply is_Some_None in Hsome; auto.
+  Qed.
+
+  Lemma state_interp_no_inv : state_interp_no_inv_type.
+  Proof. done. Qed.
+
+  Lemma crash_inner_inv : crash_inner_inv_type.
+  Proof.
+    iIntros (??) "Hinner".
+    iPoseProof (eRT.crash_inner_inv with "Hinner") as "Hinv".
+    eauto.
+  Qed.
+
+  Lemma exec_inner_inv : exec_inner_inv_type.
+  Proof.
+    iIntros (??) "Hinner".
+    iPoseProof (eRT.exec_inner_inv with "Hinner") as "Hinv".
+    eauto.
+  Qed.
+
+
+  Lemma exec_inv_preserve_finish : exec_inv_preserve_finish_type.
+  Proof.
+    iIntros (??) "Hdone Hinv".
+    iPoseProof (eRT.exec_inv_preserve_finish) as "H".
+    iMod ("H" $! _ _ with "[$] [$]") as (??) "(?&?&Hinv_post)".
+    iModIntro. iExists _, _. iFrame. iIntros.
+    iIntros (??? Hfinish ??) "((?&Hdisk)&?)".
+    inversion Hfinish. subst.
+    iMod (gen_heap_strong_init (init_zero)) as (hM Hmpf_eq) "(Hmc&Hm)".
+    iDestruct "Hdisk" as (??) "(_&?&%&%&%&%)". iFrame.
+    iModIntro.
+    iExists (ExMachG Σ (@exm_invG _ Hex) hM (@exm_disk_inG _ Hex)
+                     (@exm_treg_inG _ Hex)).
+    iSplitR "Hinv_post Hm".
+    {
+      iFrame.
+      iExists init_zero, _. iFrame.
       iPureIntro; split_and!; [ auto | auto | | assumption ].
       intros ? Hsome. apply not_le; intros Hge.
       rewrite init_zero_lookup_ge_None in Hsome; last by lia.
       apply is_Some_None in Hsome; auto.
-    - by iExists (@exm_invG _ Hex), tR.
+    }
+    iIntros "Hstate". iSpecialize ("Hinv_post" with "[Hstate Hm]").
+    { iFrame. iDestruct "Hstate" as "(?&?)". iFrame.
+      rewrite -Hmpf_eq. iApply @mem_init_to_bigOp; auto. }
+    eauto.
   Qed.
-
   End RO.
 
-  Module R := refinement RT.
+  Module R := refinement RT RO.
 
 
-  Print R.
-  Export R.
+  Export RO.
 
 End exmach_refinement.
 
-
-Section refinement.
-  Context OpT (Λa: Layer OpT).
-  Context (impl: LayerImpl ExMach.Op OpT).
-  Notation compile_op := (compile_op impl).
-  Notation compile_rec := (compile_rec impl).
-  Notation compile_seq := (compile_seq impl).
-  Notation compile := (compile impl).
-  Notation recover := (recover impl).
-  Notation compile_proc_seq := (compile_proc_seq impl).
-  Context `{exmachPreG Σ}.
-  Context `{cfgPreG OpT Λa Σ}.
-  Context (crash_inner: forall {_ : @cfgG OpT Λa Σ} {_: exmachG Σ}, iProp Σ).
-  Context (exec_inner: forall {_ : @cfgG OpT Λa Σ} {_ : exmachG Σ}, iProp Σ).
-  Context (crash_param: forall (_ : @cfgG OpT Λa Σ) (_ : exmachG Σ), Type).
-  Context (crash_inv: forall {H1 : @cfgG OpT Λa Σ} {H2 : exmachG Σ}, @crash_param _ _ → iProp Σ).
-  Context (crash_starter: forall {H1 : @cfgG OpT Λa Σ} {H2 : exmachG Σ}, @crash_param _ _ → iProp Σ).
-  Context (exec_inv: forall {_ : @cfgG OpT Λa Σ} {_ : exmachG Σ}, iProp Σ).
-
-  Context (einv_persist: forall {H1 : @cfgG OpT Λa Σ} {H2 : exmachG Σ}, Persistent (exec_inv H1 H2)).
-  Context (cinv_persist: forall {H1 : @cfgG OpT Λa Σ} {H2 : exmachG Σ}
-            {P: crash_param _ _}, Persistent (crash_inv H1 H2 P)).
-
-  Context (E: coPset).
-  Context (nameIncl: nclose sourceN ⊆ E).
-  (* TODO: we should get rid of rec_seq if we're not exploiting vertical comp anymore *)
-  Context (recv: proc ExMach.Op unit).
-  Context (recsingle: recover = rec_singleton recv).
-
-  Context (refinement_op_triples:
-             forall {H1 H2 T1 T2} j K `{LanguageCtx OpT T1 T2 Λa K} (op: OpT T1),
-               j ⤇ K (Call op) ∗ Registered ∗ (@exec_inv H1 H2) ⊢
-                 WP compile (Call op) {{ v, j ⤇ K (Ret v) ∗ Registered }}).
-
-  Context (exec_inv_source_ctx: ∀ {H1 H2}, exec_inv H1 H2 ⊢ source_ctx).
-
-  Lemma refinement_triples:
-             forall {H1 H2 T1 T2} j K `{LanguageCtx OpT T1 T2 Λa K} (e: proc OpT T1),
-               wf_client e →
-               j ⤇ K e ∗ Registered ∗ (@exec_inv H1 H2) ⊢
-                 WP compile e {{ v, j ⤇ K (Ret v) ∗ Registered }}.
-  Proof.
-    intros.
-    epose (@refinement_triples _ _ _ _ _ exmachG).
-    rewrite /RefinementIdempotence.exmachG in b.
-    simpl.
-    eapply @refinement_triples with (exmachG' := exmachG).
-
-
-    . (exmachG := exmachG Σ)). with (exmachG := exmachG Σ)).
-
-
-
-    intros ???? j K Hctx e Hwf.
-    iIntros "(Hj&Hreg&#Hinv)".
-    iAssert (⌜∃ ea: State Λa, True⌝)%I as %[? _].
-    {
-      iDestruct (exec_inv_source_ctx with "Hinv") as ((?&?)) "#Hctx".
-      eauto.
-    }
-    assert (Inhabited (State Λa)).
-    { eexists. eauto. }
-    assert (Inhabited Λa.(OpState)).
-    { eexists. destruct x; eauto. }
-    iInduction e as [] "IH" forall (j T2 K Hctx).
-    - iApply refinement_op_triples; iFrame; eauto.
-    - wp_ret. iFrame.
-    - wp_bind.
-      iApply wp_wand_l. iSplitL ""; last first.
-      * unshelve (iApply ("IH1" $! _ _ _ (fun x => K (Bind x p2)) with "[] Hj"); try iFrame).
-        { eapply Hwf. }
-        { iPureIntro. apply comp_ctx; auto. apply _. }
-      * iIntros (?) "(Hj&Hreg)".
-        iDestruct (exec_inv_source_ctx with "Hinv") as "#Hctx".
-        iMod (ghost_step_bind_ret with "Hj []") as "Hj".
-        { set_solver+. }
-        { eauto. }
-        iApply ("IH" with "[] [] Hj Hreg"); auto.
-        { iPureIntro. eapply Hwf. }
-    - iLöb as "IHloop" forall (init Hwf).
-      iDestruct (exec_inv_source_ctx with "Hinv") as "#Hctx".
-      iMod (ghost_step_loop with "Hj []") as "Hj".
-      { set_solver+. }
-      { eauto. }
-      wp_loop.
-      iApply wp_wand_l.
-      iSplitL ""; last first.
-      * rewrite /loop1. simpl.
-        unshelve (iApply ("IH" $! _ _ _ _ (fun x => K (Bind x
-                               (fun out => match out with
-                               | ContinueOutcome x => Loop body x
-                               | DoneWithOutcome r => Ret r
-                               end))) with "[] Hj Hreg")%proc).
-        { eauto. }
-        { iPureIntro. apply comp_ctx; auto. apply _. }
-      * iIntros (out) "(Hj&Hreg)".
-        destruct out.
-        ** iNext.
-           iMod (ghost_step_bind_ret with "Hj []") as "Hj".
-           { set_solver+. }
-           { eauto. }
-           iApply ("IHloop" with "[] Hj Hreg").
-           { eauto. }
-        ** iNext.
-           iMod (ghost_step_bind_ret with "Hj []") as "Hj".
-           { set_solver+. }
-           { eauto. }
-           wp_ret. iFrame.
-   - inversion Hwf.
-   - inversion Hwf.
-   - iDestruct (exec_inv_source_ctx with "Hinv") as "#Hctx".
-     iMod (ghost_step_spawn with "Hj []") as "(Hj&Hj')".
-     { set_solver+. }
-     { eauto. }
-     iDestruct "Hj'" as (j') "Hj'".
-     iApply (wp_spawn with "Hreg [Hj'] [Hj]").
-     { iNext. iIntros "Hreg'". 
-       { wp_bind.
-         iApply (wp_wand with "[Hj' Hreg'] []").
-         { unshelve (iApply ("IH" $! _ _ _ (fun x => Bind x (fun _ => Unregister))
-                               with "[] Hj' Hreg'")).
-           { eauto. }
-           { iPureIntro. apply _. }
-         }
-         { iIntros (?) "(?&?)". iApply (wp_unregister with "[$]"). iIntros "!> ?". eauto. }
-       }
-     }
-     iIntros "!> ?". iFrame.
-  Qed.
-
-  Context (recv_triple:
-             forall {H1 H2} param,
-               (@crash_inv H1 H2 param) ∗ Registered ∗ (@crash_starter H1 H2 param) ⊢
-                    WP recv @ NotStuck; ⊤ {{ v, |={⊤,E}=> ∃ σ2a σ2a', source_state σ2a
-                    ∗ ⌜Λa.(crash_step) σ2a (Val σ2a' tt)⌝ ∗
-                    ∀ `{Hcfg': cfgG OpT Λa Σ} (Hinv': invG Σ) tr',
-                      source_ctx ∗ source_state σ2a'  ={⊤}=∗
-                      exec_inner Hcfg' (ExMachG Σ Hinv' exm_mem_inG exm_disk_inG tr')
-                                               }}).
-
-  Context (init_absr: Λa.(OpState) → ExMach.State → Prop).
-  Context (init_wf: ∀ σ1a σ1c, init_absr σ1a σ1c → state_wf σ1c).
-
-  Context (init_exec_inner: ∀ σ1a σ1c, init_absr σ1a σ1c →
-      (∀ `{Hex: exmachG Σ} `{Hcfg: cfgG OpT Λa Σ},
-          (([∗ map] i ↦ v ∈ mem_state σ1c, i m↦ v) ∗
-           ([∗ map] i ↦ v ∈ disk_state σ1c, i d↦ v) ∗
-           source_ctx ∗ source_state σ1a) ={⊤}=∗ exec_inner _ _)).
-
-  Context (exec_inv_preserve_crash:
-      (∀ `{Hex: exmachG Σ} `{Hcfg: cfgG OpT Λa Σ},
-          exec_inv Hcfg Hex ={⊤, E}=∗ ∀ Hmem' Hreg',
-          (let Hex := ExMachG Σ (exm_invG) Hmem' (exm_disk_inG) Hreg' in
-              ([∗ map] i ↦ v ∈ init_zero, i m↦ v) ={E}=∗ crash_inner Hcfg Hex))).
-
-  Context (crash_inv_preserve_crash:
-      (∀ `{Hex: exmachG Σ} `{Hcfg: cfgG OpT Λa Σ} param,
-          crash_inv Hcfg Hex param ={⊤, E}=∗ ∀ Hmem' Hreg',
-          (let Hex := ExMachG Σ (exm_invG) Hmem' (exm_disk_inG) Hreg' in
-              ([∗ map] i ↦ v ∈ init_zero, i m↦ v) ={E}=∗ crash_inner Hcfg Hex))).
-
-  (* TODO: Much of this business is just to capture the fact that exec_inner/crash_inner
-     should not really mention invariants, because those old invariants are 'dead' *)
-  Context (crash_inner_inv :
-      (∀ `{Hex: exmachG Σ} `{Hcfg: cfgG OpT Λa Σ},
-          (∃ Hinv, crash_inner Hcfg (ExMachG Σ Hinv (exm_mem_inG) (exm_disk_inG) (exm_treg_inG))) ∗
-          source_ctx ={⊤}=∗ ∃ param, crash_inv Hcfg Hex param ∗ crash_starter Hcfg Hex param)).
-
-  Context (exec_inner_inv :
-      (∀ `{Hex: exmachG Σ} `{Hcfg: cfgG OpT Λa Σ},
-          (∃ Hinv, exec_inner Hcfg (ExMachG Σ Hinv (exm_mem_inG) (exm_disk_inG) (exm_treg_inG))) ∗
-          source_ctx ={⊤}=∗ exec_inv Hcfg Hex)).
-
-  Context (exec_inv_preserve_finish:
-      (∀ `{Hex: exmachG Σ} `{Hcfg: cfgG OpT Λa Σ},
-          AllDone -∗ exec_inv Hcfg Hex ={⊤, E}=∗ ∃ (σ2a σ2a' : Λa.(OpState)), source_state σ2a
-          ∗ ⌜Λa.(finish_step) σ2a (Val σ2a' tt)⌝ ∗
-          ∀ `{Hcfg': cfgG OpT Λa Σ} (Hinv': invG Σ) Hmem' Hreg',
-            (let Hex := ExMachG Σ Hinv' Hmem' (exm_disk_inG) Hreg' in
-            source_ctx∗ source_state σ2a' ∗ ([∗ map] i ↦ v ∈ init_zero, i m↦ v) ={⊤}=∗
-               exec_inner Hcfg' Hex))%I).
-
-
-  Lemma exmach_crash_refinement_seq {T} σ1c σ1a (es: proc_seq OpT T) :
-    init_absr σ1a σ1c →
-    wf_client_seq es →
-    ¬ proc_exec_seq Λa es (rec_singleton (Ret ())) (1, σ1a) Err →
-    ∀ σ2c res, proc_exec_seq ExMach.l (compile_proc_seq es)
-                                        (rec_singleton recv) (1, σ1c) (Val σ2c res) →
-    ∃ σ2a, proc_exec_seq Λa es (rec_singleton (Ret tt)) (1, σ1a) (Val σ2a res).
-  Proof.
-    rewrite /compile_proc_seq. intros Hinit Hwf_seq Hno_err σ2c0 ?.
-    unshelve (eapply wp_proc_seq_refinement_adequacy with
-                  (Λc := l)
-                  (φ := fun va vc _ _ => ⌜ va = vc ⌝%I)
-                  (E0 := E); eauto).
-    clear Hno_err.
-  iAssert (∀ invG H1 ρ, |={⊤}=>
-       ∃ hM hD tR
-            (Hmpf_eq : hM.(@gen_heap_inG addr nat Σ nat_eq_dec nat_countable) =
-          H.(@exm_preG_disk Σ).(@gen_heap_preG_inG addr nat Σ nat_eq_dec nat_countable))
-            (Hdpf_eq : hD.(@gen_heap_inG addr nat Σ nat_eq_dec nat_countable) =
-          H.(@exm_preG_disk Σ).(@gen_heap_preG_inG addr nat Σ nat_eq_dec nat_countable)),
-         (@ex_mach_interp _ hM hD {| treg_name := tR; treg_counter_inG := _ |} (1, σ1c)) ∗
-         (source_ctx' (ρ, σ1a) -∗ source_state σ1a ={⊤}=∗
-         own tR (Cinl (Count (-1))) ∗ 
-          exec_inner H1 (ExMachG Σ invG hM hD {| treg_name := tR; treg_counter_inG := _ |})))%I
-      as "Hpre".
-  {
-  iIntros.
-  iMod (gen_heap_strong_init (mem_state σ1c)) as (hM Hmpf_eq) "(Hmc&Hm)".
-  iMod (gen_heap_strong_init (disk_state σ1c)) as (hD Hdpf_eq) "(Hdc&Hd)".
-  iMod (own_alloc (Cinl (Count 0))) as (tR) "Ht".
-  { constructor. }
-  set (tR' := {| treg_name := tR; treg_counter_inG := _ |}).
-  iAssert (own tR (Cinl (Count 1)) ∗ own tR (Cinl (Count (-1))))%I with "[Ht]" as "(Ht&Hreg)".
-  { rewrite /Registered -own_op Cinl_op counting_op' //=. }
-  iModIntro. iExists hM, hD, tR, Hmpf_eq, Hdpf_eq. iSplitL "Hmc Hdc Ht".
-  { iFrame. iExists _, _. iFrame. iPureIntro.
-    edestruct (init_wf) as (Hwf1&Hwf2); eauto.
-    split_and!; eauto; intros i.
-    * destruct (Hwf1 i); intuition.
-    * destruct (Hwf2 i); intuition.
-  }
-  iIntros.
-  iPoseProof (init_exec_inner σ1a σ1c Hinit (ExMachG Σ _ hM hD tR') _) as "H".
-  iMod ("H" with "[-Hreg]") as "$".
-  { iFrame.  iSplitL "Hm"; [| iSplitL "Hd"].
-    { rewrite -Hmpf_eq. iApply mem_init_to_bigOp; auto. }
-    { rewrite -Hdpf_eq. iApply disk_init_to_bigOp; auto. }
-    iExists _; eauto.
-  }
-  iFrame; eauto.
-  }
-
-  clear Hinit.
-  iInduction es as [|es] "IH" forall (σ1a σ1c) "Hpre"; first by eauto.
-  - iSplit; first by eauto.
-  iExists (fun cfgG s => ∃ (Hex : exmachG Σ), state_interp s ∗
-            (∃ (hM: gen_heapG addr nat Σ) tr
-               (Hmpf_eq : hM.(@gen_heap_inG addr nat Σ nat_eq_dec nat_countable) =
-                          H.(@exm_preG_disk Σ).(@gen_heap_preG_inG addr nat Σ
-                                                                   nat_eq_dec nat_countable))
-               (Hdpf_eq : (@exm_disk_inG Σ Hex).(@gen_heap_inG addr nat Σ
-                                                               nat_eq_dec nat_countable)=
-                          H.(@exm_preG_disk Σ).(@gen_heap_preG_inG addr nat Σ
-                                                                   nat_eq_dec nat_countable)) ,
-            gen_heap_ctx init_zero ∗ own tr (Cinl (Count 0)) ∗ crash_inner cfgG (ExMachG Σ _ hM (exm_disk_inG) {| treg_name := tr; treg_counter_inG := _ |})))%I; auto.
-  iIntros (invG0 Hcfg0).
-  iMod ("Hpre" $! invG0 _ _) as (hM hD tr ??) "(Hstate0&H)".
-  set (tR' := {| treg_name := tr; treg_counter_inG := _ |}).
-  iExists (@ex_mach_interp _ hM hD tR').
-  iIntros "!> (#Hsrc&Hpt0&Hstate)".
-  iMod ("H" with "Hsrc Hstate") as "(Hreg&Hinv)".
-  iMod (exec_inner_inv (ExMachG Σ _ hM hD tR') _ with "[Hinv]") as "#Hinv".
-  { iSplitR ""; last by (iExists _; iFrame). iExists _. iFrame. }
-  simpl.
-  iModIntro.
-  iFrame "Hstate0".
-  iSplitL "Hpt0 Hreg".
-  {  iPoseProof (@wp_mono with "[Hpt0 Hreg]") as "H"; swap 1 2.
-     { iApply @refinement_triples. destruct (Hwf_seq) as (?&?). eauto. iFrame. iFrame "Hinv".
-       iFrame "Hreg".
-     }
-     { reflexivity. }
-     simpl. rewrite /compile_whole.
-     wp_bind.
-     iApply (wp_wand with "H [Hinv]").
-     iIntros (v) "(Hpt0&Hreg)". iFrame.
-     wp_bind.
-     iApply (@wp_wait Σ {| exm_invG := invG0;
-             exm_mem_inG := hM;
-             exm_disk_inG := hD;
-             exm_treg_inG := tR' |}
-               with "Hreg").
-     iIntros "!> Hdone".
-     wp_ret. iFrame. iExists _. iFrame. iIntros (σ2c) "Hmach".
-     iMod (exec_inv_preserve_finish with "Hdone Hinv") as (σ2a σ2a') "(H&Hfina&Hfinish)".
-     iDestruct "Hfina" as %Hfina.
-     iModIntro. iExists _; iFrame; auto.
-     simpl.
-     rewrite -/wp_proc_seq_refinement.
-     iIntros (σ2c'). iIntros.
-     unshelve (iExists σ2a', _); [eauto |]; [].
-     iApply "IH".
-     { iPureIntro. destruct Hwf_seq. eauto. }
-     { iIntros.
-       iMod (gen_heap_strong_init (init_zero)) as (hM' Hmpf_eq') "(Hmc&Hm)".
-       iMod (own_alloc (Cinl (Count 0))) as (tR_fresh') "Ht".
-       { constructor. }
-       iAssert (own tR_fresh' (Cinl (Count 1))
-                    ∗ own tR_fresh' (Cinl (Count (-1))))%I with "[Ht]" as "(Ht&Hreg)".
-       { rewrite /Registered -own_op Cinl_op counting_op' //=. }
-       set (tR''' := {| treg_name := tR_fresh'; treg_counter_inG := _ |}).
-       iModIntro.
-       iExists hM'. iExists hD. iExists tR_fresh'. unshelve (iExists _, _); try eauto.
-       destruct σ2c as (n&σ2c). iDestruct "Hmach" as "(?&Hmach)".
-       iFrame.
-       iSplitL ("Hmc Hmach").
-       { iClear "IH". iDestruct "Hmach" as (mem0 disk) "(?&?&%&%&%&%)".
-         iExists init_zero, disk. iFrame.
-         inversion Hfinish. subst. rewrite /crash_fun. simpl.
-         iPureIntro. split_and!; [ | | apply init_state_wf |]; auto.
-       }
-       iIntros "Hctx' Hsrc'". iMod ("Hfinish" $! _ _ hM' with "[-]").
-       iSplitL "Hctx'"; first by (iExists _; iFrame). iFrame.
-       { rewrite -Hmpf_eq'. iApply (@mem_init_to_bigOp _ (ExMachG Σ _ hM' hD tR') with "Hm"). }
-       iFrame; eauto.
-     }
-  }
-  iSplit.
-  { iIntros (σ2c) "Hmach".
-    iMod (exec_inv_preserve_crash with "Hinv") as "Hinv_post".
-    iMod (gen_heap_strong_init (init_zero)) as (hM' Hmpf_eq') "(Hmc&Hm)".
-    iMod (own_alloc (Cinl (Count 0))) as (tR_fresh') "Ht".
-    { constructor. }
-    set (tR''' := {| treg_name := tR_fresh'; treg_counter_inG := _ |}).
-    iMod ("Hinv_post" with "[Hm]") as "Hinv'".
-    { rewrite -Hmpf_eq'. iApply @mem_init_to_bigOp; auto. }
-    iIntros. iModIntro.
-    iExists (ExMachG Σ _ hM hD tR'). iFrame "Hmach".
-    iExists hM', tR_fresh', Hmpf_eq', H2. iFrame.
-  }
-  iClear "Hsrc".
-  iModIntro. iIntros (invG Hcfg' ?? Hcrash) "(Hinv0&#Hsrc)".
-  iDestruct "Hinv0" as (HexmachG') "(Hinterp&Hinv0)".
-  iDestruct "Hinv0" as (hM' tR_fresh' Hmpf_eq' Hmdpf_eq') "(Hmc'&Hreg&Hcrash_inner)".
-  iClear "Hinv".
-  set (tR''' := {| treg_name := tR_fresh'; treg_counter_inG := _ |}).
-  iMod (crash_inner_inv (ExMachG Σ _
-                                 hM' (exm_disk_inG) tR''') Hcfg'
-                         with "[Hcrash_inner]") as (param) "(#Hinv&Hstarter)".
-  { iIntros. simpl. iSplitR ""; last by (iExists _; iFrame).
-    iExists ( exmachG_irisG.(@iris_invG Op _ Σ)).
-    iFrame. }
-  iModIntro.
-  iAssert (own tR_fresh' (Cinl (Count 1)) ∗ own tR_fresh' (Cinl (Count (-1))))%I
-    with "[Hreg]" as "(Ht&Hreg)".
-  { rewrite /Registered -own_op Cinl_op counting_op' //=. }
-  iExists (@ex_mach_interp Σ hM' (exm_disk_inG) tR''').
-  iSplitL "Hinterp Ht Hmc'".
-  { (* shows ex_mach_interp is holds after crash for next gen *)
-    rewrite /ex_mach_interp'.
-    rewrite /ex_mach_interp.
-    destruct a, a0.
-    iDestruct "Hinterp" as "(?&Hinterp)".
-    iDestruct "Hinterp" as (mems disks) "(Hdisks&?&%&Hp)".
-    iDestruct "Hp" as %(Hdisks&Hwf1'&Hwf2').
-    destruct Hcrash as ([]&(?&?)&Hput&Hrest).
-    inversion Hput. inversion H4. subst.
-    inversion Hrest; subst. inversion H3. subst.
-    iSplitL "Ht".
-    { iFrame. }
-    iExists init_zero, _.
-    iFrame.
-    iPureIntro. split_and!.
-    * rewrite /crash_fun//=.
-    * rewrite /crash_fun//=.
-    * rewrite /crash_fun/=. intros i Hsome.
-      apply not_le; intros Hge.
-      rewrite init_zero_lookup_ge_None in Hsome; last by lia.
-      apply is_Some_None in Hsome; auto.
-    * rewrite /crash_fun; auto.
-  }
-  iSplitL "Hinv Hreg Hstarter".
-  {
-    iPoseProof (@wp_mono with "[Hinv Hreg Hstarter IH]") as "H"; swap 1 2.
-    { iApply recv_triple. iFrame "Hstarter". iFrame. iApply "Hinv". }
-    { reflexivity. }
-    iApply (@wp_wand with "H [IH]").
-    iIntros (_) "H". iIntros (σ2c) "Hinterp".
-    iMod "H". iModIntro.
-    iDestruct "H" as (σ2a σ2a') "(Hsource&Hinner&Hfinish)".
-    iExists (1, σ2a), (1, σ2a'). iFrame.
-     rewrite -/wp_proc_seq_refinement.
-     iDestruct "Hinner" as %?.
-     iSplitL "".
-     { iPureIntro. exists tt, (1, σ2a); split; eauto. econstructor. split; eauto. eauto.
-       econstructor; eauto.
-     }
-     iApply "IH".
-     { destruct Hwf_seq. eauto. }
-     { iIntros.
-       iMod (own_alloc (Cinl (Count 0))) as (tR_fresh'') "Ht".
-       { constructor. }
-       iAssert (own tR_fresh'' (Cinl (Count 1))
-                    ∗ own tR_fresh'' (Cinl (Count (-1))))%I with "[Ht]" as "(Ht&Hreg)".
-       { rewrite /Registered -own_op Cinl_op counting_op' //=. }
-       set (tR'''' := {| treg_name := tR_fresh''; treg_counter_inG := _ |}).
-       iModIntro.
-       iExists hM'. iExists (HexmachG'.(@exm_disk_inG Σ)). iExists tR_fresh''.
-       unshelve (iExists _; iExists _); eauto.
-       destruct σ2c. iDestruct "Hinterp" as "(?&?)".
-       iFrame. iIntros. iMod ("Hfinish" with "[-]"). iSplitL ""; first by (iExists _; iFrame).
-       iFrame. eauto.
-     }
-  }
-  {
-    iIntros (σ2c) "Hmach".
-    iMod (crash_inv_preserve_crash with "Hinv") as "Hinv_post".
-    iMod (gen_heap_strong_init (init_zero)) as (hM'' Hmpf_eq'') "(Hmc&Hm)".
-    iMod (own_alloc (Cinl (Count 0))) as (tR_fresh'') "Ht".
-    { constructor. }
-    set (tR'''' := {| treg_name := tR_fresh''; treg_counter_inG := _ |}).
-    iMod ("Hinv_post" with "[Hm]") as "Hinv'".
-    { rewrite -Hmpf_eq''. iApply @mem_init_to_bigOp; auto. }
-    iIntros. iModIntro.
-
-    iExists {| exm_invG := invG;
-               exm_mem_inG := hM';
-               exm_disk_inG := HexmachG'.(@exm_disk_inG Σ);
-               exm_treg_inG := tR''' |}.
-    iFrame "Hmach".
-    iFrame. unshelve (iExists hM'', tR_fresh'', Hmpf_eq'', _); eauto. iFrame.
-  }
-  Qed.
-
-End refinement.
